theories/simplang/primitive_laws.v
@@ -325,7 +325,7 @@ Qed.
 Lemma sim_call e_t e_s v_t v_s f :
   to_val e_t = Some v_t →
   to_val e_s = Some v_s →
-  ⊢ Ω v_t v_s -∗ Call (#f f) e_t ⪯{Ω} Call (#f f) e_s {{ Ω }}.
+  ⊢ Ω v_t v_s -∗ Call (## f) e_t ⪯{Ω} Call (## f) e_s {{ Ω }}.
 Proof.
   intros <-%of_to_val <-%of_to_val.
   (* FIXME use lifting lemma for this *)
@@ -336,16 +336,16 @@ Proof.
 Qed.
 
 (** Coinduction support *)
-Lemma sim_while_while b_t b_s c_t c_s Inv Ψ :
-  Inv -∗
-  □ (Inv -∗
+Lemma sim_while_while b_t b_s c_t c_s inv Ψ :
+  inv -∗
+  □ (inv -∗
     (if: c_t then b_t ;; while: c_t do b_t od else #())%E ⪯{Ω}
     (if: c_s then b_s ;; while: c_s do b_s od else #())%E
-      [{ λ e_t e_s, Ψ e_t e_s ∨ (⌜e_t = while: c_t do b_t od%E⌝ ∗ ⌜e_s = while: c_s do b_s od%E⌝ ∗ Inv) }]) -∗
+      [{ λ e_t e_s, Ψ e_t e_s ∨ (⌜e_t = while: c_t do b_t od%E⌝ ∗ ⌜e_s = while: c_s do b_s od%E⌝ ∗ inv) }]) -∗
   (while: c_t do b_t od ⪯{Ω} while: c_s do b_s od [{ Ψ }])%E.
 Proof.
   iIntros "Hinv_init #Hstep".
-  iApply (sim_lift_head_coind _ (λ e_t e_s, ⌜e_t = while: c_t do b_t od%E⌝ ∗ ⌜e_s = while: c_s do b_s od%E⌝ ∗ Inv)%I with "[] [Hinv_init]"); first last.
+  iApply (sim_lift_head_coind _ (λ e_t e_s, ⌜e_t = while: c_t do b_t od%E⌝ ∗ ⌜e_s = while: c_s do b_s od%E⌝ ∗ inv)%I with "[] [Hinv_init]"); first last.
   { iFrame. eauto. }
   iModIntro. iIntros (?? ?? ??) "(-> & -> & Hinv) (Hstate & Hnreach)".
   iModIntro. iSplitR; first by eauto with head_step.
@@ -357,15 +357,15 @@ Proof.
 Qed.
 
 
-Lemma sim_while_rec b_t c_t v_s (K_s : ectx) (Inv : val → iProp Σ) Ψ rec_n :
-  Inv v_s -∗
+Lemma sim_while_rec b_t c_t v_s (K_s : ectx) (inv : val → iProp Σ) Ψ rec_n :
+  inv v_s -∗
   rec_n @s K_s -∗
-  □ (∀ v_s', Inv v_s' -∗
+  □ (∀ v_s', inv v_s' -∗
     (if: c_t then b_t ;; while: c_t do b_t od else #())%E ⪯{Ω} (fill K_s v_s')%E
-    [{ λ e_t e_s , Ψ e_t e_s ∨ (∃ v_s', ⌜e_t = while: c_t do b_t od%E⌝ ∗ ⌜e_s = Call #f rec_n (Val v_s')⌝ ∗ Inv v_s') }]) -∗
-  (while: c_t do b_t od ⪯{Ω} Call #f rec_n v_s [{ Ψ }])%E.
+    [{ λ e_t e_s , Ψ e_t e_s ∨ (∃ v_s', ⌜e_t = while: c_t do b_t od%E⌝ ∗ ⌜e_s = Call ##rec_n (Val v_s')⌝ ∗ inv v_s') }]) -∗
+  (while: c_t do b_t od ⪯{Ω} Call ## rec_n v_s [{ Ψ }])%E.
 Proof.
-  iIntros "Hinv #Hrec #Hstep". iApply (sim_lift_head_coind _ (λ e_t e_s, (∃ v_s', ⌜e_t = while: c_t do b_t od%E⌝ ∗ ⌜e_s = Call #f rec_n (Val v_s')⌝ ∗ Inv v_s')%I)); first last.
+  iIntros "Hinv #Hrec #Hstep". iApply (sim_lift_head_coind _ (λ e_t e_s, (∃ v_s', ⌜e_t = while: c_t do b_t od%E⌝ ∗ ⌜e_s = Call ##rec_n (Val v_s')⌝ ∗ inv v_s')%I)); first last.
   { iExists v_s. eauto. }
   iModIntro. iIntros (?? ?? ??) "He (Hstate & Hnreach)". iDestruct "He" as (v_s') "(-> & -> & Hinv)".
   iSpecialize ("Hstep" with "Hinv").
@@ -378,15 +378,15 @@ Proof.
   iFrame. by eauto with head_step.
 Qed.
 
-Lemma sim_rec_while b_s c_s v_t (K_t : ectx) (Inv : val → iProp Σ) Ψ rec_n :
-  Inv v_t -∗
+Lemma sim_rec_while b_s c_s v_t (K_t : ectx) (inv : val → iProp Σ) Ψ rec_n :
+  inv v_t -∗
   rec_n @t K_t -∗
-  □ (∀ v_t', Inv v_t' -∗
+  □ (∀ v_t', inv v_t' -∗
     (fill K_t v_t')%E ⪯{Ω}  (if: c_s then b_s ;; while: c_s do b_s od else #())%E
-    [{ λ e_t e_s , Ψ e_t e_s ∨ (∃ v_t', ⌜e_t = Call #f rec_n (Val v_t')⌝ ∗ ⌜e_s = while: c_s do b_s od%E⌝ ∗  Inv v_t') }]) -∗
-  ( Call #f rec_n v_t ⪯{Ω} while: c_s do b_s od [{ Ψ }])%E.
+    [{ λ e_t e_s , Ψ e_t e_s ∨ (∃ v_t', ⌜e_t = Call ##rec_n (Val v_t')⌝ ∗ ⌜e_s = while: c_s do b_s od%E⌝ ∗  inv v_t') }]) -∗
+  ( Call ##rec_n v_t ⪯{Ω} while: c_s do b_s od [{ Ψ }])%E.
 Proof.
-  iIntros "Hinv #Hrec #Hstep". iApply (sim_lift_head_coind _ (λ e_t e_s, (∃ v_t', ⌜e_t = Call #f rec_n (Val v_t')⌝ ∗ ⌜e_s = while: c_s do b_s od%E⌝ ∗  Inv v_t'))%I); first last.
+  iIntros "Hinv #Hrec #Hstep". iApply (sim_lift_head_coind _ (λ e_t e_s, (∃ v_t', ⌜e_t = Call ##rec_n (Val v_t')⌝ ∗ ⌜e_s = while: c_s do b_s od%E⌝ ∗  inv v_t'))%I); first last.
   { iExists v_t. eauto. }
   iModIntro. iIntros (?? ?? ??) "He (Hstate & Hnreach)". iDestruct "He" as (v_s') "(-> & -> & Hinv)".
   iSpecialize ("Hstep" with "Hinv").
